ROOT
@@ -1,0 +1,12 @@
+session Verified_Consensus = Word_Lib +
+  options [document = false, quick_and_dirty]
+  directories
+    "algebra/rg-algebra/AbstractAtomicTest/"
+    "algebra/rg-algebra/General" 
+    "algebra/rg-algebra/AbstractAtomic" 
+    "algebra/rg-algebra/AbstractTests"
+    "jormungand/Hoare_Sep_Tactics"
+    "jormungand/sep_algebra" 
+  theories
+    "algebra/rg-algebra/AbstractAtomicTest/Idle"
+    "jormungand/Hoare_Sep_Tactics/Extended_Separation_Algebra"
